\documentclass[11pt]{article}
\usepackage{graphicx} % more modern
%\usepackage{times}
\usepackage{helvet}
\usepackage{courier}
\usepackage{epsf}
\usepackage{amsmath,amssymb,amsfonts,verbatim}
\usepackage{subfigure}
\usepackage{amsfonts}
\usepackage{amsmath}
\usepackage{amsthm}
\usepackage{latexsym}
\usepackage{algpseudocode}
\usepackage{algorithm}
\usepackage{enumerate}
%\usepackage{algorithmic}
\usepackage{multirow}
\usepackage{xcolor}

\def\A{{\bf A}}
\def\a{{\bf a}}
\def\B{{\bf B}}
\def\b{{\bf b}}
\def\C{{\bf C}}
\def\c{{\bf c}}
\def\D{{\bf D}}
\def\d{{\bf d}}
\def\E{{\bf E}}
\def\e{{\bf e}}
\def\F{{\bf F}}
\def\f{{\bf f}}
\def\G{{\bf G}}
\def\g{{\bf g}}
\def\k{{\bf k}}
\def\K{{\bf K}}
\def\H{{\bf H}}
\def\I{{\bf I}}
\def\L{{\bf L}}
\def\M{{\bf M}}
\def\m{{\bf m}}
\def\n{{\bf n}}
\def\N{{\bf N}}
\def\BP{{\bf P}}
\def\R{{\bf R}}
\def\BS{{\bf S}}
\def\s{{\bf s}}
\def\t{{\bf t}}
\def\T{{\bf T}}
\def\U{{\bf U}}
\def\u{{\bf u}}
\def\V{{\bf V}}
\def\v{{\bf v}}
\def\W{{\bf W}}
\def\w{{\bf w}}
\def\X{{\bf X}}
\def\Y{{\bf Y}}
\def\Q{{\bf Q}}
\def\x{{\bf x}}
\def\y{{\bf y}}
\def\Z{{\bf Z}}
\def\z{{\bf z}}
\def\0{{\bf 0}}
\def\1{{\bf 1}}


\def\hx{\hat{\bf x}}
\def\tx{\tilde{\bf x}}
\def\ty{\tilde{\bf y}}
\def\tz{\tilde{\bf z}}
\def\hd{\hat{d}}
\def\HD{\hat{\bf D}}

\def\MA{{\mathcal A}}
\def\MF{{\mathcal F}}
\def\MR{{\mathcal R}}
\def\MG{{\mathcal G}}
\def\MI{{\mathcal I}}
\def\MN{{\mathcal N}}
\def\MO{{\mathcal O}}
\def\MT{{\mathcal T}}
\def\MX{{\mathcal X}}
\def\SW{{\mathcal {SW}}}
\def\MW{{\mathcal W}}
\def\MY{{\mathcal Y}}
\def\BR{{\mathbb R}}
\def\BP{{\mathbb P}}
\def\BE{{\mathbb E}}

\def\bet{\mbox{\boldmath$\beta$\unboldmath}}
\def\epsi{\mbox{\boldmath$\epsilon$}}

\def\etal{{\em et al.\/}\,}
\def\tr{\mathrm{tr}}
\def\rk{\mathrm{rk}}
\def\diag{\mathrm{diag}}
\def\dg{\mathrm{dg}}
\def\argmax{\mathop{\rm argmax}}
\def\argmin{\mathop{\rm argmin}}
\def\vecd{\mathrm{vec}}

\def\ph{\mbox{\boldmath$\phi$\unboldmath}}
\def\vp{\mbox{\boldmath$\varphi$\unboldmath}}
\def\pii{\mbox{\boldmath$\pi$\unboldmath}}
\def\Ph{\mbox{\boldmath$\Phi$\unboldmath}}
\def\pss{\mbox{\boldmath$\psi$\unboldmath}}
\def\Ps{\mbox{\boldmath$\Psi$\unboldmath}}
\def\muu{\mbox{\boldmath$\mu$\unboldmath}}
\def\Si{\mbox{\boldmath$\Sigma$\unboldmath}}
\def\lam{\mbox{\boldmath$\lambda$\unboldmath}}
\def\Lam{\mbox{\boldmath$\Lambda$\unboldmath}}
\def\Gam{\mbox{\boldmath$\Gamma$\unboldmath}}
\def\Oma{\mbox{\boldmath$\Omega$\unboldmath}}
\def\De{\mbox{\boldmath$\Delta$\unboldmath}}
\def\de{\mbox{\boldmath$\delta$\unboldmath}}
\def\Tha{\mbox{\boldmath$\Theta$\unboldmath}}
\def\tha{\mbox{\boldmath$\theta$\unboldmath}}

\newtheorem{theorem}{Theorem}[section]
\newtheorem{lemma}{Lemma}[section]
\newtheorem{definition}{Definition}[section]
\newtheorem{proposition}{Proposition}[section]
\newtheorem{corollary}{Corollary}[section]
\newtheorem{example}{Example}[section]


\def\probin{\mbox{\rotatebox[origin=c]{90}{$\vDash$}}}

\def\calA{{\cal A}}



%this is a comment

%use this as a template only... you may not need the subsections,
%or lists however they are placed in the document to show you how
%do it if needed.


%THINGS TO REMEMBER
%to compile a latex document - latex filename.tex
%to view the document        - xdvi filename.dvi
%to create a ps document     - dvips filename.dvi
%to create a pdf document    - dvipdf filename.dvi
%{\bf TEXT}                  - bold font TEXT
%{\it TEXT}                  - italic TEXT
%$ ... $                     - places ... in math mode on same line
%$$ ... $$                   - places ... in math mode on new line
%more info at www.cs.wm.edu/~mliskov/cs423_fall04/tex.html


\setlength{\oddsidemargin}{.25in}
\setlength{\evensidemargin}{.25in}
\setlength{\textwidth}{6in}
\setlength{\topmargin}{-0.4in}
\setlength{\textheight}{8.5in}


%%%%%%%%%%%%%%%%%%%%%%%%%%%%%%%%%%%%%%%%%%%%%%%%%%%%%%%%%%%%%%%%%%%%%%%%%%%%%%%%%%%
\newcommand{\notes}[5]{
	\renewcommand{\thepage}{#1 - \arabic{page}}
	\noindent
	\begin{center}
	\framebox{
		\vbox{
		\hbox to 5.78in { { \bf Statistical Machine Learning}
		\hfill #2}
		\vspace{4mm}
		\hbox to 5.78in { {\Large \hfill #5 \hfill} }
		\vspace{2mm}
		\hbox to 5.78in { {\it #3 \hfill #4} }
		}
	}
	\end{center}
	\vspace*{4mm}
}

\newcommand{\ho}[5]{\notes{#1}{Distributions}{Professor: Zhihua Zhang}{}{Lecture Notes #1: Scale Mixture Distribution}}
%%%%%%%%%%%%%%%%%%%%%%%%%%%%%%%%%%%%%%%%%%%%%%%%%%%%%%%%%%%%%%%%%%%%%%%%%%%%%%%%%%

%begins a LaTeX document
\setcounter{section}{2}
\setcounter{subsection}{3}
\begin{document}
\ho{3}{2014.03.08}{Moses Liskov}{Name}{Lecture title}
\textbf{Notice:} In this lecture note, $X \sim \MN(a,b)$ means that $\mu=a,\sigma^2=b$. Prof.Zhang sometimes means $\mu=a,\sigma=b$ in the class. So the notation or results may be a little different with your notes.

\subsection{Scale Mixture Distribution}
We will show several distributions can be seen as the scale mixture of distributions, which is defined as follows,
\[\begin{split}
  X \sim F(\theta) \\
  \theta \sim G(\lambda)
\end{split}\],
So, $T(x) = \int_{\theta} F(\theta) G(\lambda) d\theta$ can be seen as a scale mixture of $F$, where the scale has distribution $G$.

\subsubsection{Student's t-distribution}
The Student's t-distribution is a scale mixture of Gaussian distribution, where the scale has a Gamma distribution. 
Let $X \sim \MN(\mu, \frac{\sigma^2}{r})$, $r \sim\mbox{Gamma}(\frac{\nu}{2},\frac{\nu}{2})$, then the integral will be:
\[\begin{split}  &  \int_0^{\infty} \frac{r^{1/2}}{\sqrt{2\pi}\sigma} e^{-\frac{r(x-\mu)^2}{2\sigma^2}}  
\frac{(\frac{\nu}{2})^{\frac{\nu}{2}}}{\Gamma{(\frac{\nu}{2}})} r^{\frac{\nu}{2}-1} e^{-\frac{\nu}{2}r} \mathrm{d}r \\
= & \frac{(\frac{\nu}{2})^{\frac{\nu}{2}}}{\Gamma{(\frac{\nu}{2})}\sigma\sqrt{2\pi}}
\int_0^\infty r^{\frac{\nu+1}{2} - 1} 
e^{-\frac{r}{2}(\frac{(x-\mu)^2}{\sigma^2} + \nu)}  \mathrm{d}r \\
= & \frac{(\frac{\nu}{2})^{\frac{\nu}{2}}\Gamma{(\frac{\nu+1}{2})}}{\sigma\sqrt{2\pi}\Gamma{(\frac{\nu}{2})}} 
\left[\frac{(x-\mu)^2}{\sigma^2} + \nu\right]^{-\frac{\nu+1}{2}} \\
= & \frac{\Gamma{(\frac{\nu+1}{2})}}{\sigma\sqrt{\nu\pi}\Gamma{(\frac{\nu}{2})}} 
\left[\frac{(x-\mu)^2}{\nu\sigma^2} + 1\right]^{-\frac{\nu+1}{2}} \\
= & t_\nu(\mu,\sigma^2)
\end{split}\]

Note that during the integral, we use a mathematical trick. Since we have $$\int_0^\infty \frac{\beta^\alpha}{\Gamma(\alpha)} x^{\alpha - 1} e^{-\beta x} dx = 1$$ from Gamma distribution, so we can get 
$\int_0^\infty x^{\alpha - 1} e^{-\beta x} dx = \frac{\Gamma(\alpha)}{\beta^\alpha}$. 
This trick will be often used in the follows.

\subsubsection{Laplace Distribution}
Laplace distribution is:
$$f(x) = \frac{1}{4\sigma}\exp(-\frac{|x-\mu|}{2\sigma})$$
Let we see $2\sigma$ as $\sigma$ for convenience, that is:
$$f(x) = \frac{1}{2\sigma}\exp(-\frac{|x-\mu|}{\sigma})$$
The Laplace distribution is a scale mixture of Gaussian distribution, where the scale has a exponential distribution.
Let $X \sim \MN(\mu, r)$, $r \sim \mbox{Exponential}(\frac{1}{2\sigma^2})$, then we can get the mixture distribution:
\[\begin{split} &
\int_0^\infty \frac{1}{\sqrt{2\pi r}} e^{-\frac{(x-\mu)^2}{2r}}
\frac{1}{2\sigma^2} e^{-\frac{r}{2\sigma^2}} \mathrm{d}r  \\
 = & \frac{1}{2\sigma^2 \sqrt{2\pi}}  \int_0^\infty
 r^{\frac{1}{2} - 1} e^{-\frac{1}{2} \left( \frac{(x-\mu)^2}{r} + \frac{r}{\sigma^2}\right)} \mathrm{d}r  \\
 = & \frac{1}{2\sigma^2 \sqrt{2\pi}} \frac{2K_{1/2}\left(\sqrt{(\frac{1}{\sigma^2}(x-\mu)^2)}\right)}{(\frac{1}{\sigma^2(x-\mu)^2})^{\frac{1}{4}}} \\
 = &\frac{1}{2\sigma} e^{\frac{|x-\mu|}{\sigma}}
\end{split}\]
The integral term is a integral of generalized inverse Gaussian distribution, $\mbox{GIG}(\frac{1}{2},\frac{1}{\sigma^2},(x-\mu)^2)$.

\subsubsection{Negative Binomial Distribution}
Negative Binomial Distribution is a scale of Poisson distribution, where the scale has a Gamma distribution.
Let $K \sim \mbox{Poisson}(\lambda)$, $\lambda \sim \mbox{Gamma}(r, \frac{1-p}{p})$, then we can get the mixture distribution:
\[\begin{split}
&  \int_0^\infty \frac{\lambda^k}{k!} e^{-\lambda}
\frac{\lambda^{r-1} e^{-\frac{1-p}{p} \lambda}}{\Gamma(r) (\frac{p}{1-p})^r} \mathrm{d}\lambda \\
= & \frac{1}{k! \Gamma(r) (\frac{p}{1-p})^r}  \int_0^\infty  \lambda^{k+r-1}  e^{-\frac{\lambda}{p}} \mathrm{d}\lambda \\
=&\frac{\Gamma(r+k)p^k(1-p)^r}{\Gamma(k)\Gamma(r)}\\
= & {k+r-1 \choose k} p^k (1-p)^r
\end{split}\]

\textbf{Homework 1:}   $\sum\limits_{k=0}^\infty \mbox{Gamma}(x | k+p, \beta) \mbox{Poisson} (k | \lambda),  p\mbox{ is a postive constant}$.

\section{Statistical Inference (I)}

\subsection{Jeffreys Prior}
In order to show Jeffrey prior, we first introduce \textbf{Fisher information}. In mathematical statistics, the Fisher information is a way of measuring the amount of information that an observable random variable $X$ carries about an unknown parameter $\theta$ upon which the probability of $X$ depends.

The probability function for $X$, which is also the likelihood function for $\theta$, is a function $f(X; \theta)$; it is the probability mass (or probability density) of the random variable $X$ conditional on the value of $\theta$. Then we define Fisher information:
\begin{definition}
Fisher Information:
$$I(\theta)=\BE((\frac{\partial\log f(x; \theta)}{\partial\theta})^2)$$
\end{definition}

\begin{lemma}
If $\log f(x; \theta)$ is twice differentiable with respect to $\theta$ and under certain regularity conditions, then
$$I(\theta) = -\BE(\frac{\partial^2\log f}{\partial\theta ^ 2})$$
\end{lemma}

\begin{proof}
first
\begin{align}
\nonumber
\frac{\partial^2\log f}{\partial\theta ^ 2} &= \frac{\partial}{\partial\theta}(\frac{\frac{\partial f}{\partial\theta}}{f}) \\
\nonumber
&= \frac{\frac{\partial^2f}{\partial\theta^2}}{f} - \frac{(\frac{\partial f}{\partial\theta})^2}{f^2}\\
\nonumber
&= \frac{\frac{\partial^2f}{\partial\theta^2}}{f} - (\frac{\partial\log f}{\partial\theta}) ^ 2
\end{align}
then
\begin{align}
\nonumber
\BE(\frac{\partial^2\log f}{\partial\theta ^ 2}) &= \int\frac{\partial^2\log f}{\partial\theta^2}f \mathrm{d}x\\
\nonumber
&= \int \frac{\partial^2f}{\partial\theta^2}\mathrm{d}x - I(\theta)
\end{align}
if $\int \frac{\partial^2f}{\partial\theta^2}\mathrm{d}x = \frac{\partial^2}{d\theta^2}\int f\mathrm{d}x = \frac{\partial^2}{\partial\theta}1 = 0$(the certain condition),then we had proved the lemma.
\end{proof}
\begin{definition}
Jeffreys prior is defined in terms of Fisher information
$$p(\theta) \propto \sqrt{I(\theta)}$$
\end{definition}
\textbf{Remark:} It has the key feature that it is \textbf{invariant under reparametrization} of parameter $\theta$. For an alternate parametrization $\varphi$ we can derive
$$p(\varphi) \propto \sqrt{I(\varphi)}$$
from
$$p(\theta) \propto \sqrt{I(\theta)}$$
where $\theta$ and $\varphi$ exist a one-to-one mapping.
\begin{proof}
\begin{align}
\nonumber
p(\varphi) &= p(\theta)|\frac{d\theta}{d\varphi}| \propto \sqrt{I(\theta)(\frac{d\theta}{d\varphi})^2}
\propto\sqrt{\BE((\frac{d\log f}{d\theta})^2)(\frac{d\theta}{d\varphi})^2} \\
\nonumber
&\propto \sqrt{\BE((\frac{d\log f}{d\theta}\frac{d\theta}{d\varphi})^2)} = \sqrt{\BE((\frac{d\log f}{d\varphi})^2)} \propto \sqrt{I(\varphi)}
\end{align}
\end{proof}

\begin{example}
$X \sim \MN(\mu, \sigma^2)$.
\end{example}
\begin{description}
\item[Case 1:] Fix $\sigma$, the only parameter is $\mu$. The likelihood is:
$$f(X|\mu) \propto \exp(-\frac{1}{2\sigma^2}(x - \mu)^2)$$
so
$$\log f \propto -(\frac{x-\mu}{\sigma})^2$$So we can get:
\[\begin{split} 
I(\mu) &= \BE\left[ \left( \frac{(x - \mu)^2}{\sigma^2} \right)^2 \right] \\
&= \frac{\BE(x - \mu)^2}{\sigma^4} \\
&= \frac{1}{\sigma^2}
\end{split}\]
Thus the Jeffreys prior $p(\mu) \propto \sqrt{I(\mu)} = \frac{1}{\sigma}$. As $\sigma$ is fixed, so $p(\mu) \propto 1$.

\textbf{Remark:} Although $p(\mu) = 1$ is a improper prior, as $\int_{-\infty}^\infty 1 dx = \infty$, the posterior is proper. 
The prior is also called \textbf{uninformative prior}.

\item[Case 2:] Fix $\mu$, the only parameter is $\sigma$. For convenience, let $\tau = \frac{1}{\sigma^2}$. So $f(x) = \frac{\tau^{\frac{1}{2}}}{\sqrt{2\pi}} e^{-\frac{\tau(x-\mu)^2}{2}}$.
The likelihood is denoted by $f(\tau)$:
\begin{eqnarray*}
&f(\tau) = \frac{\tau^{\frac{1}{2}}}{\sqrt{2\pi}}\exp(-\frac{\tau(x-\mu)^2}{2})\\
\Longrightarrow & \log f \propto \frac{1}{2}\log\tau - \frac{\tau}{2}(x - \mu)^2\\
\Longrightarrow & \frac{\partial\log f}{\partial\tau} \propto \frac{1}{2\tau} - \frac{(x-\mu)^2}{2}\\
\end{eqnarray*}

Hence, 
\[\begin{split}
I(\tau) &= \BE\left[\left( \frac{\partial \log f}{\partial \tau} \right)^2\right]  \\
&= \BE\left[ \frac{1}{4} \left( \frac{1}{\tau} - (x-\mu)^2 \right)^2  \right] \\
&= \BE\left[ \frac{1}{4\tau^2} - \frac{(x - \mu)^2}{2\tau} + \frac{(x-\mu)^4}{4} \right] \\
&= \frac{1}{4\tau^2} - \frac{1}{2\tau^2} + \frac{1}{4}\BE(x-\mu)^4 \\
&= \frac{1}{4\tau^2}-\frac{1}{2\tau^2} + \int^\infty_{-\infty} \frac{1}{4}(x - \mu)^4\MN(x|\mu, \tau^{-1})dx \\
&= \frac{1}{2\tau^2}
\end{split}\]
where the integral can be computed from variance :
\[\begin{split}
& \int (x-\mu)^2\frac{\tau^{\frac{1}{2}}}{\sqrt{2\pi}}\exp(-\frac{\tau(x-\mu)^2}{2})dx =  \tau^{-1} \\
\Longrightarrow & \int (x-\mu)^2\frac{1}{\sqrt{2\pi}}\exp(-\frac{\tau(x-\mu)^2}{2})dx =  \tau^{-\frac{3}{2}} \\ 
& \mbox{(taking the derivate of both side)} \\
\Longrightarrow & \int (x-\mu)^4\frac{1}{\sqrt{2\pi}}\exp(-\frac{\tau(x-\mu)^2}{2})dx =  3\tau^{-\frac{5}{2}} \\ 
\Longrightarrow & \int (x-\mu)^4\frac{\tau^{\frac{1}{2}}}{\sqrt{2\pi}}\exp(-\frac{\tau(x-\mu)^2}{2})dx =  3\tau^{-2} \\ 
\Longrightarrow & \BE\left((x-\mu)^4\right) = \frac{3}{4\tau^2} \\
\end{split}\]

So Jeffreys prior is $\pi(\tau) \propto\frac{1}{\tau}$.
Note that $p(\sigma)=\pi(\tau)|d\tau/d\theta|$, hence, 
\begin{eqnarray*}
p(\sigma)
\propto &\frac{1}{\tau}|-2\sigma^{-3}|\\
\propto & \sigma^2|-2\sigma^{-3}| \\
\propto & \frac{1}{\sigma} \\
\end{eqnarray*}
\end{description}
\textbf{Homework 2:} Compute the following integrals:
\begin{enumerate}
\item $u_0 = \int_{-\infty}^{\infty} \Phi(x) \MN(x|\mu, \sigma^2) dx$
\item $u_1 = \int_{-\infty}^{\infty} \Phi(x) \MN(x|\mu, \sigma^2)x dx$
\item $u_2 = \int_{-\infty}^{\infty} \Phi(x) \MN(x|\mu, \sigma^2)(x-m_1) dx$

where $\Phi(x) = \int_{-\infty}^{x} \frac{1}{\sqrt{2\pi}} e^{-\frac{t^2}{2}} dt$
\end{enumerate}

\begin{example}
$X \sim \mbox{Poisson}(n;\lambda)$
\end{example}
$$
\log f = -\lambda + n\log\lambda
$$
Fisher information is:
\[\begin{split}
I(\lambda) &= \BE\left[ \left( \frac{n}{\lambda} - 1\right)^2 \right] \\
&= 1 + \frac{\BE(n^2)}{\lambda^2} - 2 \\
&= \frac{\lambda + 1}{\lambda} - 1 \\
&= \frac{1}{\lambda}
\end{split}\]
So Jeffreys prior is:
\[\begin{split}
p(\lambda) \propto \sqrt{\frac{1}{\lambda}}.
\end{split}\]
 
\textbf{Homework 3:} $f(x; \theta) = \theta^x(1-\theta)^{1-x}$, $0 < \theta < 1$.
\begin{enumerate}
\item Compute Jeffreys prior about $\theta$.
\item If $\theta = \sin^2 \alpha$, compute Jeffreys prior about $\alpha$.
\end{enumerate}
 
\subsection{Compute Posterior Probability}
Assume we have a model $x = \theta + \epsilon$, where $x$ is data which we observed or predict, $\theta$ is the parameters, $\epsilon \sim \MN(0, \tau)$ is the error term. So given $\theta$, $X \sim \MN(\theta, \tau)$. When we use MAP(maximum a posteriori) to estimate parameter $\theta$, we will get $p(\theta | x) \propto p(x | \theta)p(\theta)$. 
We will discuss this problem under several different conditions in the following.
\begin{description}
\item[Case 1] Fix $\tau$. The only parameter is $\theta$. And we set the prior about $\theta$ is $\MN(\theta | 0, \lambda)$. So
\[\begin{split} 
p(\theta | x) &\propto p(x | \theta) p(\theta) \\
&\propto \frac{1}{\sqrt{2\pi\tau}} e^{-\frac{(x - \theta)^2}{2\tau}} 
\frac{1}{\sqrt{2\pi\lambda}} e^{-\frac{\theta^2}{2\lambda}} \\
&\propto \frac{1}{2\pi \sqrt{\tau\lambda}} e^{-\frac{1}{2} [(\frac{1}{\tau} + \frac{1}{\lambda})( \theta - \frac{\lambda x}{\tau + \lambda} )^2 + \frac{x^2}{\tau + \lambda}] } \\
&\propto \MN(\frac{\lambda x}{\lambda+\tau},\frac{\lambda\tau}{\lambda+\tau})
\end{split}\]
Then we can get the estimation about $\theta$ from MAP, $\hat{\theta} = \frac{\lambda x}{\lambda + \tau}$.

\item[Case 2] Let $\theta$ and $\tau$ both be parameters. In order to get MAP, we may make three solutions.

\begin{description}
    \item[Solution 1]Assume that $\tau$, $\lambda$ are independent. $p(\theta, \tau) = p(\theta)p(\tau)$
    and we use a new $\tau$ here, $\tau = \tau_{old}^{-1}$ for convenience of computing(It is different with the $\tau$ used in case 1). Suppose $\tau \thicksim \mbox{Gamma}(\alpha/2, \beta/2)$
    \begin{eqnarray*}
    p(\theta, \tau|x) &\propto p(x| \theta, \tau) p(\theta, \tau) = p(x|\theta, \tau)p(\theta)p(\tau)
    \nonumber\\
    &\propto \frac{1}{\sqrt{2\pi}}\tau^\frac{1}{2}\exp(-\frac{\tau(x-\theta)^2}{2})\frac{\lambda^\frac{1}{2}}{\sqrt{2\pi}}
    \exp(-\frac{\lambda\theta^2}{2})(\frac{\beta}{2})^\frac{\alpha}{2}\exp(-\frac{\beta \tau}{2})\frac{\tau ^{\frac{\alpha}{2} - 1}}{\Gamma(\alpha/2)}
    \end{eqnarray*}
    To get maximum posterior, let
    $$L = \tau^{\frac{\alpha+1}{2}-1}\lambda^\frac{1}{2}\exp(-\frac{\tau}{2}((x-\theta)^2+\beta)-\frac{\lambda\theta^2}{2})$$
    then
    $$\ln L = (\frac{\alpha+1}{2}-1)\ln\tau - \frac{\tau}{2}((x-\theta)^2+\beta) + \frac{1}{2}\ln\lambda -\frac{\lambda\theta^2}{2}$$
    Let
    $$Q = -2\ln L = -(\alpha - 1)\ln\tau + \tau((x-\theta)^2+\beta) - \ln\lambda + \lambda\theta^2$$
    We need to solve equations:
    \begin{equation*}
      \begin{cases}
        \frac{\partial Q}{\partial\theta} &= -2\tau(x-\theta) + 2\lambda\theta = 0 \\
        \frac{\partial Q}{\partial\tau} &= \frac{1-\alpha}{\tau} + (x -\theta)^2 + \beta = 0
      \end{cases}
    \end{equation*}
It is a difficult problem to solve, especially when $\theta$ is a vector.

\textbf{Remark :} One way to solve the problem above is to compute one parameter, for example $\theta$, while fixing the other parameter, i.e. $\tau$. Then fix $\theta$, compute $\theta$. Hold on until they get convergent. Well, then we need to think about the convergence problem.

\item[Solution 2] Assume $p(\theta, \tau)=p(\theta|\tau)p(\tau)$, and $p(\theta |\tau) \sim \MN(0, (\lambda\tau)^{-1})$, suppose $\tau \thicksim \mbox{Gamma}(\alpha/2, \beta/2)$, follow the same steps in solution 1, we get:
\[\begin{split}
p(\theta, \tau | x) &\propto p(x | \theta, \tau) p(\theta | \tau) p(\tau) \\
&\propto \frac{\tau^{\frac{1}{2}}}{\sqrt{2\pi}} e^{-\frac{\tau(x-\theta)^2}{2}}
\frac{(\lambda \tau)^{\frac{1}{2}}}{\sqrt{2\pi}} e^{-\frac{\lambda\tau\theta^2}{2}}
(\frac{\beta}{2})^\frac{\alpha}{2}e^{(-\frac{\beta \tau}{2})}\frac{\tau ^{\frac{\alpha}{2} - 1}}{\Gamma(\alpha/2)}
\end{split}
\]
Then the corresponding $L$ is given by:
    $$L = \tau^{\frac{\alpha+1}{2}-1}(\lambda\tau)^\frac{1}{2}\exp(-\frac{\tau}{2}((x-\theta)^2+\beta)-\frac{\lambda\tau\theta^2}{2}).$$
Then the $Q$ is
$$Q = -2\ln L = -(\alpha - 1)\ln\tau + \tau((x-\theta)^2+\beta) - \ln(\lambda\tau) + \lambda\tau\theta^2$$
To get the estimation of $\theta$ and $\tau$, we need to solve:
\[\begin{cases}
\frac{\partial Q}{\partial \theta} = 0 \\
\frac{\partial Q}{\partial \tau} = 0
\end{cases}
\]
Then we will get:
\begin{equation*} \begin{cases}
-\tau(x-\theta)+\tau\lambda = 0  \\
\beta - \frac{\alpha - 1}{\tau} - \frac{1}{\tau}+(x-\theta)^2 + \lambda\theta^2= 0 \\
\end{cases}
\end{equation*}
We can easily solve $\theta$ and $\tau$. It is called \textbf{decouple}.

\item[Solution 3] From the two sub-cases above, we can find the major problem is computing complexity. Another problem will occurs if there are too many hyper-parameters. As we need to search the best hyper-parameters by grid search. So if there are 2 hyper-parameters, the search space is 2-dimensional. If there are 3 hyper-parameters, the search space is 3-dimensional... It will cost too much time when the search space is high dimensional.

Simply, we can give an uninformative prior to $\tau$, $p(\tau) \propto 1$. Or we can consider Jeffreys prior for $\tau$. According to Example 3.1, case 2,we get $p(\tau)\propto \frac{1}{\tau}$. So we will have:
\[\begin{split}
p(\theta, \tau | x) &\propto p(x | \theta, \tau) p(\theta | \tau) p(\tau) \\
&\propto \frac{1}{\sqrt{2\pi\tau}} e^{-\frac{(x-\theta)^2}{2\tau}} \frac{1}{\sqrt{2\pi\lambda\tau}} e^{-\frac{\theta^2}{2\lambda\tau}} \frac{1}{\tau}=L \\
\end{split}\]
Removing constants, we will get:
\[ Q = -2\ln L = 3\ln\tau + \ln(\lambda\tau) + \frac{(x-\theta)^2}{\tau} + \frac{\theta^2}{\lambda\tau} \]
Then according to $\frac{\partial Q}{\partial \theta} = 0$ and $\frac{\partial Q}{\partial \tau} = 0$, we will get the followings:
\[\begin{cases}
-2(x-\theta)+\frac{2\theta}{\lambda} = 0 \\
\frac{3}{\tau}+\frac{1}{\tau}-\frac{1}{\tau^2}\left(\frac{(x-\theta)^2}{2}+\frac{\theta^2}{\lambda}\right) = 0 \\
\end{cases}\]
We can see it is easy to solve and there is no extra parameter.(Solution 2 has two new parameters, $\alpha$ and $\beta$)
\end{description}
\end{description}
\end{document}




